src/named/PfCompilers.v
@@ -6,54 +6,118 @@ Unset Printing Implicit Defensive.
 Set Bullet Behavior "Strict Subproofs".
 
 From Utils Require Import Utils.
-From Named Require Import Pf PfCore.
+From Named Require Import Pf PfCoreDefs.
 Require Import String.
 
 
-(* each element is the image for that constructor *)
-Definition compiler := named_list pf. 
+(* each element is the image for that constructor or axiom*)
+Variant compiler_case := con_case (e:wfexp) | ax_case (p : pf).
+Definition compiler := named_list compiler_case. 
 
 (*TODO: find right place for this *)
 Definition get_rule_ctx r :=
   match r with
-  | sort_rule_pf c _
-  | term_rule_pf c _ _
-  | sort_le_pf c _ _
-  | term_le_pf c _ _ _ => c
+  | Pf.wf_sort_rule c _
+  | Pf.wf_term_rule c _ _
+  | wf_sort_le c _ _
+  | wf_term_le c _ _ _ => c
   end.
 
 Section CompileFn.
-  Context (l : pf_lang) (*TODO: use pflang? makes no difference*)
+  Context (src tgt : wfexp_lang)
           (cmp : compiler).
 
-  Fixpoint compile (e : pf) : pf :=
+  (*TODO: add args to compiler case so that lang argument is unnecessary?*)
+  Fixpoint compile (e : wfexp) : wfexp :=
     match e with
-    | pvar x => pvar x
-    | pcon n s =>
-      let default := pcon "ERR" [::] in
-      let default_r := sort_rule_pf [::] [::] in
+    | wf_var x => wf_var x
+    | wf_con n s =>
+      let default := wf_con "ERR" [::] in
+      let default_r := Pf.wf_sort_rule [::] [::] in
       let arg_terms := map compile s in
-      let constr_pf := named_list_lookup default cmp n in
-      let c := get_rule_ctx (named_list_lookup default_r l n) in
-      pf_subst (with_names_from c arg_terms) constr_pf
-    (*TODO: unify ax and pcon?*)
-    | ax n s =>
-      let default := pcon "ERR" [::] in
-      let default_r := sort_rule_pf [::] [::] in
-      let arg_terms := map compile s in
-      let constr_pf := named_list_lookup default cmp n in
-      let c := get_rule_ctx (named_list_lookup default_r l n) in
-      pf_subst (with_names_from c arg_terms) constr_pf
-    | sym p => sym (compile p)
-    | trans p1 p2 => trans (compile p1) (compile p2)
-    | conv pt p => conv (compile pt) (compile p)
-    end.
-
+      let c := get_rule_ctx (named_list_lookup default_r src n) in
+      let case := named_list_lookup (con_case default) cmp n in
+      match case with
+      | con_case e => wfexp_subst (with_names_from c arg_terms) e
+      | _ => default
+      end
+    | wf_conv pt p => wf_conv (compile_pf pt) (compile p)
+    end
+  with compile_pf (e : pf) : pf :=
+         match e with
+         | ax n =>
+           let default := ax "ERR" in
+           match named_list_lookup_err cmp n  with
+           | Some (ax_case p) => p
+           | _ => default
+           end
+         | pf_refl e => pf_refl (compile e)
+         | sym p => sym (compile_pf p)
+         | trans p1 p2 => trans (compile_pf p1) (compile_pf p2)
+         | pf_conv pt p => pf_conv (compile_pf pt) (compile_pf p)
+         | pf_subst s p => pf_subst (named_map compile_pf s) (compile_pf p)
+         end.
+  
   Definition compile_args := map compile.
 
-  Definition compile_subst (s : named_list pf) := named_map compile s.
+  Definition compile_subst (s : named_list wfexp) := named_map compile s.
 
-  Definition compile_ctx (c:named_list pf) := named_map compile c.
+  Definition compile_ctx (c:named_list wfexp) := named_map compile c.
+
+   (* First we specify the properties semantically,
+     then inductively on the compiler. TODO: prove equivalent
+   *)
+  Definition sort_wf_preserving_sem :=
+    forall c t, wf_sort src c t ->
+                wf_sort tgt (compile_ctx c) (compile t).
+
+  Definition term_wf_preserving_sem :=
+    forall c e t,
+      wf_term src c e t ->
+      wf_term tgt (compile_ctx c) (compile e) (compile t).
+
+  Definition sort_le_preserving_sem :=
+    forall c p t1 t2,
+      le_sort src c p t1 t2 ->
+      le_sort tgt (compile_ctx c) (compile_pf p)
+              (compile t1) (compile t2).
+  
+  Definition term_le_preserving_sem :=
+    forall c p t e1 e2,
+      le_term src c p t e1 e2 ->
+      le_term tgt (compile_ctx c) (compile_pf p)
+              (compile t) (compile e1) (compile e2).
+
+  Definition args_wf_preserving_sem :=
+    forall c c' s' args es es' c2 c2',
+      ctx_compiles_to c c' ->
+      args_compile_to c es c2 es' ->
+      ctx_compiles_to c2 c2' ->
+      size args = size s' ->
+      subseq (zip args s') (with_names_from c2' es') ->
+      wf_args tgt c' s' args es' c2'.
+
+
+  Definition args_le_preserving_sem :=
+    forall c c' s1' s2' args es1 es2 es1' es2' c2 c2',
+      ctx_compiles_to c c' ->
+      args_compile_to c es1 c2 es1' ->
+      args_compile_to c es2 c2 es2' ->
+      ctx_compiles_to c2 c2' ->
+      size args = size s1' ->
+      subseq (zip args s1') (with_names_from c2' es1') ->
+      size args = size s2' ->
+      subseq (zip args s2') (with_names_from c2' es2') ->
+      le_args tgt c' c2' s1' s2' args es1' es2'.
+
+  Definition ctx_wf_preserving_sem :=
+    forall c c',
+      ctx_compiles_to c c' ->
+      wf_ctx tgt c'.
+
+  Definition semantics_preserving :=
+    sort_wf_preserving_sem /\ term_wf_preserving_sem /\ args_wf_preserving_sem
+    /\ sort_le_preserving_sem /\ term_le_preserving_sem /\ args_le_preserving_sem.
 
 End CompileFn.
 
@@ -64,37 +128,34 @@ of elaborated compilers.
 
 (*TODO: this is an equal or stronger property (which?); includes le principles;
   formalize the relationship to those above and le semantic statements *)
-Inductive preserving_compiler (target : pf_lang) : compiler -> pf_lang -> Prop :=
+Inductive preserving_compiler (target : wfexp_lang) : compiler -> wfexp_lang -> Prop :=
 | preserving_compiler_nil : preserving_compiler target [::] [::]
 | preserving_compiler_sort : forall cmp l n c args t,
     preserving_compiler target cmp l ->
     (* Notable: only uses the previous parts of the compiler on c *)
-    sort_ok target (compile_ctx l cmp c) t ->
-    is_exp t ->
-    preserving_compiler target ((n, t)::cmp) ((n,sort_rule_pf c args) :: l)
+    wf_sort target (compile_ctx l cmp c) t ->
+    preserving_compiler target ((n,con_case t)::cmp) ((n,Pf.wf_sort_rule c args) :: l)
 | preserving_compiler_term : forall cmp l n c args e t,
     preserving_compiler target cmp l ->
     (* Notable: only uses the previous parts of the compiler on c, t *)
-    term_ok target (compile_ctx l cmp c) e (compile l cmp t) ->
-    is_exp e ->
-    (*is_exp t ->should I have this here? prob. not*)
-    preserving_compiler target ((n, e)::cmp) ((n,term_rule_pf c args t) :: l)
+    wf_term target (compile_ctx l cmp c) e (compile l cmp t) ->
+    preserving_compiler target ((n, con_case e)::cmp) ((n,Pf.wf_term_rule c args t) :: l)
 | preserving_compiler_sort_le : forall cmp l n c teq t1 t2,
     preserving_compiler target cmp l ->
     (* Notable: only uses the previous parts of the compiler on c *)
-    sort_ok target (compile_ctx l cmp c) teq ->
-    compile l cmp t1 = proj_l target teq ->
-    compile l cmp t2 = proj_r target teq ->
-    preserving_compiler target ((n,teq)::cmp) ((n,sort_le_pf c t1 t2) :: l)
+    le_sort target (compile_ctx l cmp c) teq (compile l cmp t1) (compile l cmp t2) ->
+    preserving_compiler target ((n,ax_case teq)::cmp) ((n,wf_sort_le c t1 t2) :: l)
 | preserving_compiler_term_le : forall cmp l n c eeq e1 e2 t,
     preserving_compiler target cmp l ->
     (* Notable: only uses the previous parts of the compiler on c *)
-    term_ok target (compile_ctx l cmp c) eeq (compile l cmp t) ->
-    compile l cmp e1 = proj_l target eeq ->
-    compile l cmp e2 = proj_r target eeq ->
-    preserving_compiler target ((n,eeq)::cmp) ((n,term_le_pf c e1 e2 t) :: l).
+    le_term target (compile_ctx l cmp c) eeq
+            (compile l cmp t) (compile l cmp e1) (compile l cmp e2) ->
+    preserving_compiler target ((n,ax_case eeq)::cmp) ((n,wf_term_le c e1 e2 t) :: l).
 
-(* TODO: decision procedure  for is_exp; move to Pf *)
+(* TODO: recover decision procedure?
+   will probably use tactics for now, but I'll eventually want this
+   for efficiency
+
 Fixpoint check_preserving tgt (cmp:compiler) src : bool :=
   match cmp, src with
   | [::], [::] => true
@@ -122,6 +183,7 @@ Fixpoint check_preserving tgt (cmp:compiler) src : bool :=
     (check_preserving tgt cmp' src')
   | _, _ => false
   end.
+*)
 
 
 Lemma fresh_compile_ctx x s cmp c
@@ -151,7 +213,8 @@ Proof.
   intro h; inversion h.
 Qed.
 Hint Resolve false_False : pfcore.
-  
+
+(*
 Lemma check_preservingP
   : forall t cmp s, all_fresh t ->
                     check_lang_ok s ->
@@ -218,7 +281,7 @@ Proof.
     end ||
         match goal with [|-?P] => idtac P end)).
 Qed.
-
+*)
 
 
 (*
